\documentclass{article}

\usepackage{amsmath}

\newcommand{\Fib}[1][]{\ensuremath{\text{Fib}(#1)}}
\newcommand{\tif}{\ensuremath{\text{if} \;}}
\newcommand{\s}{\sqrt{5}}

\begin{document}

\[
	\begin{aligned}
		a_1 &= b_0q + a_0q + a_0p \\
		b_1 &= b_0p + a_0q \\
		a_2 &= b_1q + a_1q + a_1p \\
		b_2 &= b_1p + a_1q
	\end{aligned}
\]

\[
	\begin{aligned}
		a_2 &= (b_0p + a_0q)q + (b_0q + a_0q + a_0p)q + (b_0q + a_0q + a_0p)p \\
		b_2 &= (b_0p + a_0q)p + (b_0q + a_0q + a_0p)q
	\end{aligned}
\]

Let's do $a_2$ first.

\[
	\begin{aligned}
		a_2 &= (b_0p + a_0q)q + (b_0q + a_0q + a_0p)q + (b_0q + a_0q + a_0p)p \\
		a_2 &= b_0pq + a_0q^2 + b_0q^2 + a_0q^2 + a_0pq + b_0pq + a_0pq + a_0p^2 \\
		a_2 &= b_0pq +  b_0q^2 + b_0pq +  a_0q^2  + a_0q^2 + a_0pq +  a_0pq + a_0p^2 \\
		a_2 &= b_0(q^2 + 2pq) + a_0(q^2 + 2pq)  + a_0(p^2 + q^2)
	\end{aligned}
\]

Now we should have $q' = q^2 + 2pq$ and $p' = p^2 + q^2$, and this should check
out on the $b$ transformation.

\[
	\begin{aligned}
		b_2 &= (b_0p + a_0q)p + (b_0q + a_0q + a_0p)q \\
		b_2 &= b_0p^2 + a_0pq + b_0q^2 + a_0q^2 + a_0pq \\
		b_2 &= b_0p^2 + b_0q^2 + 2a_0pq + a_0q^2  \\
		b_2 &= b_0(p^2 + q^2) + a_0(q^2 + 2pq) \\
		b_2 &= b_0p' + a_0q' \\
	\end{aligned}
\]

\end{document}
