\documentclass{article}

\usepackage{amsmath}

\begin{document}

\newcommand \w[0]{\text{width}}
\renewcommand \c[0]{\text{center}}
\renewcommand \t[0]{\text{tolerance}}

\[
   \begin{aligned}
      \, [a, b] \cdot [c, d] = \left[
         \min(ac, ad, bc, bd), 
         \max(ac, ad, bc, bd)
      \right]
   \end{aligned}
\]

Assuming that all numbers are positive

\[
   \begin{aligned}
      \, [a, b] \cdot [c, d] = \left[ ac, bd \right]
   \end{aligned}
\]

Lets find the exact formula:

\[
   \begin{aligned}
      \w([ac, bd]) &= \frac{ac - bd}{2}. \\
      \c([ac, bd]) &= \frac{ac + bd}{2}. \\
      \t([ac, bd]) &= \frac{\w([ac, bd])}{\c([ac,bd])} \\
         &= \frac{
            \frac{ac - bd}{2}
         }{
            \frac{ac + bd}{2}
         } \\
         & = \frac{ac - bd}{2}
             \frac{2}{ac + bd} \\
         & = \frac{ac - bd}{ac + bd} \\
   \end{aligned}
\]

\[
   \begin{aligned}
      \t([a, b]) &= \frac{a - b}{a + b} \\
      \t([c, d]) &= \frac{c - d}{c + d} \\
   \end{aligned}
\]
\[
   \begin{aligned}
      \frac{a - b}{a + b} + \frac{c - d}{c + d} & = 
      \frac{(a - b)(c + d)}{(a + b)(c + d)} + \frac{(c - d)(a + b)}{(c + d)(a +
b)} \\
      = &
      \frac{ac + ad - bc - bd}{ac + ad + bc + bd} + 
      \frac{ca + cb - da - db}{ac + ad + bc + bc} \\
      = &
      \frac{2ac - 2ad}{ac + ad + bc + bd}  \\
      = 2 \frac{ac - ad}{ac + bd + ad + bc}  \\
   \end{aligned}
\]

If we assume:
\[
   \begin{aligned}
   ad \approx ac \\
   bc \approx bd
   \end{aligned}
\]

Then
\[
   \begin{aligned}
   2 \frac{ac - ad}{ac + bd + ad + bc} & \approx 2 \frac{ac - ad}{2 ac + 2 bd} \\
    & = \frac{ac - ad}{ac + bd} \\
   \end{aligned}
\]

\end{document}
